Try to get tree stuff into a file of its own

Incredible_Completeness.thy
@@ -1,319 +1,6 @@
 theory Incredible_Completeness
-imports Natural_Deduction Incredible_Deduction
+imports Natural_Deduction Incredible_Deduction Incredible_Trees
 begin
-
-lemma prefixeq_snocD: "prefixeq (xs@[x]) ys \<Longrightarrow> prefix xs ys"
-  by (simp add: prefixI' prefix_order.dual_order.strict_trans1)
-
-lemma image_eq_to_f:
-  assumes  "f1 ` S1 = f2 ` S2"
-  obtains f where "\<And> x. x \<in> S2 \<Longrightarrow> f x \<in> S1 \<and> f1 (f x) = f2 x"
-proof (atomize_elim)
-  from assms
-  have "\<forall>x. x \<in> S2 \<longrightarrow> (\<exists> y. y \<in> S1 \<and> f1 y = f2 x)" by (metis image_iff)
-  thus "\<exists>f. \<forall>x. x \<in> S2 \<longrightarrow> f x \<in> S1 \<and> f1 (f x) = f2 x" by metis
-qed
-
-context includes fset.lifting
-begin
-lemma fimage_eq_to_f:
-  assumes  "f1 |`| S1 = f2 |`| S2"
-  obtains f where "\<And> x. x |\<in>| S2 \<Longrightarrow> f x |\<in>| S1 \<and> f1 (f x) = f2 x"
-using assms apply transfer using image_eq_to_f by metis
-end
-
-
-section {* Elaborated tree (annotation and substitution) *}
-
-text {*
-Tree-shape, but incredible-graph-like content (port names, explicit annotation and substitution)
-*}
-
-datatype ('preform,'rule,'subst,'var)  itree =
-    INode (iNodeOf': "('preform, 'rule) graph_node")
-          (iOutPort': "'preform reg_out_port")
-          (iAnnot: "nat")
-          (iSubst: "'subst")
-          (iAnts': "('preform, 'var) in_port \<rightharpoonup> ('preform,'rule,'subst,'var) itree")
-  | HNode (iAnnot: "nat")
-          (iSubst: "'subst")
-
-fun iAnts where
-   "iAnts (INode n p i s ants) = ants"
- | "iAnts (HNode i s) = empty"
-
-fun iNodeOf where
-   "iNodeOf (INode n p i s ants) = n"
- | "iNodeOf (HNode i s) = Helper"
-
-context Abstract_Formulas
-begin
-fun iOutPort where
-   "iOutPort (INode n p i s ants) = p"
- | "iOutPort (HNode i s) = anyP"
-end
-
-context Abstract_Task
-begin
-  inductive iwf :: "('preform,'rule,'subst,'var) itree \<Rightarrow> 'form entailment \<Rightarrow> bool" where
-    iwf: "\<lbrakk>
-       n \<in> sset nodes;
-       Reg p |\<in>| outPorts n;
-       \<And> ip. ip |\<in>| inPorts n \<Longrightarrow>
-          (\<exists> t. ants ip = Some t \<and>
-              iwf t ((\<lambda> h . subst s (freshen i (labelsOut n h))) |`| hyps_for n ip |\<union>| \<Gamma> \<turnstile> subst s (freshen i (labelsIn n ip))));
-       \<And> ip. ip |\<in>| inPorts n  \<Longrightarrow> f |\<in>| \<Gamma> \<Longrightarrow> freshenV i ` (local_vars n ip) \<inter> fv f = {};
-       \<And> ip. ip |\<in>| inPorts n  \<Longrightarrow> freshenV i ` (local_vars n ip) \<inter> ran_fv s = {};
-       c = subst s (freshen i (labelsOut n (Reg p :: (('preform, 'var) out_port))))
-      \<rbrakk> \<Longrightarrow> iwf (INode n p i s ants) (\<Gamma> \<turnstile> c)"  
-  | iwfH: "\<lbrakk>
-       c |\<notin>| ass_forms;
-       c |\<in>| \<Gamma>;
-       c = subst s (freshen i anyP)
-      \<rbrakk> \<Longrightarrow> iwf (HNode i s) (\<Gamma> \<turnstile> c)"  
-
-
-lemma build_iwf:
-  fixes t :: "('form entailment \<times> ('rule \<times> 'preform) NatRule) tree"
-  assumes "tfinite t"
-  assumes "wf t"
-  shows "\<exists> it. iwf it (fst (root t))"
-using assms
-proof(induction)
-  case (tfinite t)
-  from `wf t`
-  have "snd (root t) \<in> R" using wf.simps by blast
-
-  from `wf t`
-  have "eff (snd (root t)) (fst (root t)) ((fst \<circ> root) |`| cont t)" using wf.simps by blast
-
-  from `wf t`
-  have "\<And> t'. t' |\<in>| cont t \<Longrightarrow> wf t'" using wf.simps by blast
-  hence IH: "\<And> \<Gamma>' t'. t' |\<in>| cont t \<Longrightarrow> (\<exists>it'. iwf it' (fst (root t')))" using tfinite(2) by blast
-  then obtain its where its: "\<And> t'. t' |\<in>| cont t \<Longrightarrow> iwf (its t') (fst (root t'))" by metis
-
-  from `eff _ _ _`
-  show ?case
-  proof(cases rule: eff.cases[case_names Axiom NatRule Cut])
-  case (Axiom con \<Gamma>)
-    show ?thesis
-    proof (cases "con |\<in>| ass_forms")
-      case True (* Global assumption *)
-      then obtain c :: "'preform" where
-        "c \<in> set assumptions" and [simp]: "subst undefined (freshen undefined c) = con"
-        by (auto simp add:  ass_forms_def)
-
-      let "?it" = "INode (Assumption c) c undefined undefined empty ::  ('preform, 'rule, 'subst, 'var) itree"
-
-      from `c \<in> set assumptions`
-      have "iwf ?it (\<Gamma> \<turnstile> con)" by (auto intro!: iwf)
-      thus ?thesis unfolding Axiom..
-    next
-      case False
-      obtain s where [simp]: "subst s (freshen undefined anyP) = con" by atomize_elim (rule anyP_is_any)
-  
-      let "?it" = "HNode undefined s ::  ('preform, 'rule, 'subst, 'var) itree"
-  
-      from  `con |\<in>| \<Gamma>` False
-      have "iwf ?it (\<Gamma> \<turnstile> con)" by (auto intro: iwfH)
-      thus ?thesis unfolding Axiom..
-    qed
-  next
-  case (NatRule rule c ants \<Gamma> i s)
-    from `natEff_Inst rule c ants`
-    have "snd rule = c"  and [simp]: "f_antecedent (fst rule) = ants" and "c \<in> set (consequent (fst rule))"
-      by (auto simp add: natEff_Inst.simps)  
-
-    from `(fst \<circ> root) |\`| cont t = (\<lambda>ant. (\<lambda>p. subst s (freshen i p)) |\`| a_hyps ant |\<union>| \<Gamma> \<turnstile> subst s (freshen i (a_conc ant))) |\`| ants`
-    obtain to_t where "\<And> ant. ant |\<in>| ants \<Longrightarrow> to_t ant |\<in>| cont t \<and> (fst \<circ> root) (to_t ant) = ((\<lambda>p. subst s (freshen i p)) |`| a_hyps ant |\<union>| \<Gamma> \<turnstile> subst s (freshen i (a_conc ant)))"
-      by (rule fimage_eq_to_f) (rule that)
-    hence to_t_in_cont: "\<And> ant. ant |\<in>| ants \<Longrightarrow> to_t ant |\<in>| cont t"
-      and to_t_root: "\<And> ant. ant |\<in>| ants \<Longrightarrow>  fst (root (to_t ant)) = ((\<lambda>p. subst s (freshen i p)) |`| a_hyps ant |\<union>| \<Gamma> \<turnstile> subst s (freshen i (a_conc ant)))"
-      by auto
-
-    let "?it" = "INode (Rule (fst rule)) c i s (\<lambda> ant. if ant |\<in>| ants then Some (its (to_t ant)) else None) ::  ('preform, 'rule, 'subst, 'var) itree"
-
-    from `snd (root t) \<in> R`
-    have "fst rule \<in> sset rules"
-      unfolding NatRule
-      by (auto simp add: stream.set_map n_rules_def no_empty_conclusions )
-    moreover
-    from `c \<in> set (consequent (fst rule))`
-    have "c |\<in>| f_consequent (fst rule)" by (simp add: f_consequent_def)
-    moreover
-    { fix ant
-      assume "ant |\<in>| ants"
-      from its[OF to_t_in_cont[OF this]]
-      have "iwf (its (to_t ant)) (fst (root (to_t ant)))".
-      also have "fst (root (to_t ant)) =
-        ((\<lambda>h. subst s (freshen i (labelsOut (Rule (fst rule)) h))) |`| hyps_for (Rule (fst rule)) ant |\<union>| \<Gamma>
-         \<turnstile> subst s (freshen i (a_conc ant)))"
-        by (auto simp add: to_t_root `ant |\<in>| ants`)
-      finally
-      have "iwf (its (to_t ant))
-           ((\<lambda>h. subst s (freshen i (labelsOut (Rule (fst rule)) h))) |`| hyps_for (Rule (fst rule)) ant |\<union>|
-            \<Gamma>  \<turnstile> subst s (freshen i (a_conc ant)))".
-    }
-    moreover
-    note NatRule(5,6)
-    ultimately
-    have "iwf ?it ((\<Gamma> \<turnstile> subst s (freshen i c)))"
-      apply -
-      apply (rule iwf)
-      apply auto
-      apply blast
-      done
-    thus ?thesis unfolding NatRule..
-  next
-  case (Cut \<Gamma> con)
-    obtain s where [simp]: "subst s (freshen undefined anyP) = con" by atomize_elim (rule anyP_is_any)
-
-    from `(fst \<circ> root) |\`| cont t = {|\<Gamma> \<turnstile> con|}`
-    obtain t'  where "t' |\<in>| cont t" and [simp]: "fst (root t') = (\<Gamma> \<turnstile> con)"
-      by (cases "cont t") auto
-    
-    from `t' |\<in>| cont t` obtain "it'" where "iwf it' (\<Gamma> \<turnstile> con)" using IH by force
-
-    let "?it" = "INode Helper anyP undefined s (empty(plain_ant anyP \<mapsto> it')) ::  ('preform, 'rule, 'subst, 'var) itree"
-
-    from `iwf it' (\<Gamma> \<turnstile> con)`
-    have "iwf ?it (\<Gamma> \<turnstile> con)" by (auto intro!: iwf)
-    thus ?thesis unfolding Cut..
-  qed 
-qed
-
-definition to_it :: "('form entailment \<times> ('rule \<times> 'preform) NatRule) tree \<Rightarrow> ('preform,'rule,'subst,'var) itree" where
-  "to_it t = (SOME it. iwf it (fst (root t)))"
-
-lemma iwf_to_it:
-  assumes "tfinite t" and "wf t"
-  shows "iwf (to_it t) (fst (root t))"
-unfolding to_it_def using build_iwf[OF assms] by (rule someI2_ex)
-
-
-  fun fv_entailment :: "'form entailment \<Rightarrow> 'var annotated set" where
-    "fv_entailment (\<Gamma> \<turnstile> c) = Union (fv ` fset \<Gamma>) \<union> fv c"
-
-  inductive iwf' :: "('preform,'rule,'subst,'var) itree \<Rightarrow> 'form entailment \<Rightarrow> bool" where
-    iwf': "\<lbrakk>
-       n \<in> sset nodes;
-       Reg p |\<in>| outPorts n;
-       \<And> ip. ip |\<in>| inPorts n \<Longrightarrow>
-          (\<exists> t. ants ip = Some t \<and>
-              iwf' t ((\<lambda> h . subst s (freshen i (labelsOut n h))) |`| hyps_for n ip |\<union>| \<Gamma> \<turnstile> subst s (freshen i (labelsIn n ip))));
-       ran_fv s \<subseteq> fv_entailment (\<Gamma> \<turnstile> c) \<union> range (freshenV i);
-       c = subst s (freshen i (labelsOut n (Reg p :: (('preform, 'var) out_port))))
-      \<rbrakk> \<Longrightarrow> iwf' (INode n p i s ants) (\<Gamma> \<turnstile> c)"  
-  | iwf'H: "\<lbrakk>
-       c |\<notin>| ass_forms;
-       c |\<in>| \<Gamma>;
-       c = subst s (freshen i anyP)
-      \<rbrakk> \<Longrightarrow> iwf' (HNode i s) (\<Gamma> \<turnstile> c)"  
-
-lemma iwf'_subst_freshen_outPort:
-  "iwf' ts ent \<Longrightarrow>
-  snd ent = subst (iSubst ts) (freshen (iAnnot ts) (iOutPort ts))"
-  by (auto elim: iwf'.cases)
-
-
-
-lemma iwf'_to_it:
-  assumes "tfinite t" and "wf t"
-  shows "iwf' (to_it t) (fst (root t))"
-sorry
-
-
-inductive it_pathsP :: "('preform,'rule,'subst,'var) itree \<Rightarrow> ('preform, 'var) in_port list \<Rightarrow> bool"  where
-   it_paths_Nil: "it_pathsP t []"
- | it_paths_Cons: "i |\<in>| inPorts (iNodeOf t) \<Longrightarrow> iAnts t i = Some t' \<Longrightarrow> it_pathsP t' is \<Longrightarrow> it_pathsP t (i#is)"
-
-inductive_cases it_pathP_ConsE: "it_pathsP t (i#is)"
-
-definition it_paths:: "('preform,'rule,'subst,'var) itree \<Rightarrow> ('preform, 'var) in_port list set"  where
-  "it_paths t = Collect (it_pathsP t)"
-
- lemma it_paths_eq [pred_set_conv]: "it_pathsP t = (\<lambda>x. x \<in> it_paths t)"
-   by(simp add: it_paths_def)
-
- lemmas it_paths_intros [intro?] = it_pathsP.intros[to_set]
- lemmas it_paths_induct [consumes 1, induct set: it_paths] = it_pathsP.induct[to_set]
- lemmas it_paths_cases [consumes 1, cases set: it_paths] = it_pathsP.cases[to_set]
- lemmas it_paths_ConsE = it_pathP_ConsE[to_set]
- lemmas it_paths_simps = it_pathsP.simps[to_set]
-
- lemma [simp]: "[] \<in> it_paths t" by (rule it_paths_intros)
-
-lemma it_paths_HNode[simp]: "it_paths (HNode i s) = {[]}"
-  by (auto elim: it_paths_cases)
-
-lemma it_paths_Union: "it_paths t \<subseteq> insert [] (Union (fset ((\<lambda> i. case iAnts t i of Some t \<Rightarrow> (op # i) ` it_paths t | None \<Rightarrow> {}) |`| (inPorts (iNodeOf t)))))"
-  apply (rule)
-  apply (subst (asm) it_paths_simps)
-  apply (fastforce split: prod.split simp add: fmember.rep_eq)
-  done
-
-lemma finite_it_paths[simp]: "finite (it_paths t)"
-  by (induction t) (rule finite_subset[OF it_paths_Union], fastforce split: option.split intro: range_eqI)+
-end
-
-fun tree_at :: "('preform,'rule,'subst,'var) itree \<Rightarrow> ('preform, 'var) in_port list \<Rightarrow> ('preform,'rule,'subst,'var) itree" where
-  "tree_at t [] = t"
-| "tree_at t (i#is) = tree_at (the (iAnts t i)) is"
-
-context Abstract_Task
-begin
-lemma it_path_SnocE[elim_format]:
-  assumes "is @ [i] \<in> it_paths t"
-  shows "is \<in> it_paths t \<and> i |\<in>| inPorts (iNodeOf (tree_at t is))"
-using assms
-by (induction "is" arbitrary: t)(auto intro!: it_paths_intros elim!: it_paths_ConsE)
-
-fun isHNode where
-  "isHNode (HNode _ _) = True"
- |"isHNode _ = False"
-
-lemma it_path_SnocI:
-  assumes "iwf' t ant"
-  assumes "is \<in> it_paths t" 
-  assumes "\<not> isHNode (tree_at t is)"
-  assumes "i |\<in>| inPorts (iNodeOf (tree_at t is))"
-  shows "is @ [i] \<in> it_paths t"
-  using assms
-  apply (induction arbitrary: "is" i)
-  apply auto
-  apply (case_tac "is")
-  apply (force intro: it_paths_intros elim!: it_paths_ConsE)+
-  done
-
-lemma iwf'_edge_match:
-  assumes "iwf' t ent"
-  assumes "is@[i] \<in> it_paths t"
-  shows "subst (iSubst (tree_at t (is@[i]))) (freshen (iAnnot (tree_at t (is@[i]))) (iOutPort (tree_at t (is@[i]))))
-     = subst (iSubst (tree_at t is)) (freshen (iAnnot (tree_at t is)) (a_conc i))"
-  using assms
-  apply (induction arbitrary: "is" i)
-  apply (case_tac "is")
-  apply (force elim!: it_paths_ConsE intro: trans[OF iwf'_subst_freshen_outPort[symmetric]])+
-  done
-
-
-lemma it_paths_prefix:
-  assumes "is \<in> it_paths t"
-  assumes "prefix is' is"
-  shows "is' \<in> it_paths t"
-proof-
-  from assms(2)
-  obtain is'' where "is = is' @ is''" using prefixE' by blast
-  from assms(1)[unfolded this]
-  show ?thesis
-    by(induction is' arbitrary: t) (auto elim!: it_paths_ConsE intro!: it_paths_intros)
-qed
-end
-
-
-type_synonym ('preform, 'var) vertex = "('preform \<times> ('preform, 'var) in_port list)"
-type_synonym ('preform, 'var) edge'' = "(('preform, 'var) vertex, 'preform, 'var) edge'"
-
 
 locale Solved_Task =
   Abstract_Task freshen pre_fv fv subst ran_fv closed anyP antecedent consequent rules assumptions conclusions
@@ -348,95 +35,77 @@ lemma
   using solved assms
   by (force simp add: solved_def)
 
-abbreviation to_form :: "'preform \<Rightarrow> 'form" where
-  "to_form pf \<equiv> subst undefined (freshen undefined pf)"
+text {* To get the list of vertices, build the tree with local freshness first. *}
 
-lemma to_form_conc_forms[simp]: "to_form a |\<in>| conc_forms \<longleftrightarrow> a \<in> set conclusions"
-proof
-  assume "a \<in> set conclusions"
-  thus "to_form a |\<in>| conc_forms" by (rule subst_freshen_in_conc_formsI)
-next
-  assume "to_form a |\<in>| conc_forms"
-  then obtain a' where "a' \<in> set conclusions" and "to_form a = to_form a'"
-    by (auto simp add: conc_forms_def)
-  thus "a \<in> set conclusions" using conclusions_closed closed_eq by metis
-qed
+abbreviation pre_it where
+  "pre_it c \<equiv> to_it (ts (to_form c))"
 
-abbreviation it where
-  "it c \<equiv> to_it (ts (to_form c))"
-
-lemma iwf'_it:
+lemma iwf_pre_it:
   assumes "c \<in> set conclusions"
-  shows "iwf' (it c) (fst (root (ts (to_form c))))"
-  using assms by (auto intro!: iwf'_to_it ts_finite ts_wf)
+  shows "local_iwf (pre_it c) (fst (root (ts (to_form c))))"
+  using assms by (auto intro!: iwf_to_it ts_finite ts_wf)
 
 definition vertices :: "('preform, 'var) vertex fset"  where
-  "vertices = Abs_fset (Union ( set (map (\<lambda> c. insert (c, []) ((\<lambda> p. (c, plain_ant c # p)) ` (it_paths (it c))))  conclusions)))"
+  "vertices = Abs_fset (Union ( set (map (\<lambda> c. insert (c, []) ((\<lambda> p. (c, plain_ant c # p)) ` (it_paths (pre_it c))))  conclusions)))"
 
-lemma mem_vertices: "v |\<in>| vertices \<longleftrightarrow>  (fst v \<in> set conclusions \<and> (snd v = [] \<or> snd v \<in> (op # (plain_ant (fst v))) ` it_paths (it (fst v))))"
+text {* For the remaining time, work with the tree with global freshness. *}
+
+abbreviation it' where
+  "it' c \<equiv> globalize (to_it (ts (to_form c)))"
+
+lemma mem_vertices: "v |\<in>| vertices \<longleftrightarrow>  (fst v \<in> set conclusions \<and> (snd v = [] \<or> snd v \<in> (op # (plain_ant (fst v))) ` it_paths (it' (fst v))))"
   unfolding vertices_def fmember.rep_eq ffUnion.rep_eq 
-  by (cases v) (auto simp add: Abs_fset_inverse Bex_def)
+  by (cases v)(auto simp add: Abs_fset_inverse Bex_def it_paths_globalize)
 
 lemma none_vertices[simp]: "(c, []) |\<in>| vertices \<longleftrightarrow> c \<in> set conclusions"
   by (simp add: mem_vertices)
 
-lemma some_vertices[simp]: "(c, i#is) |\<in>| vertices \<longleftrightarrow> c \<in> set conclusions \<and> i = plain_ant c \<and> is \<in> it_paths (it c)"
+lemma some_vertices[simp]: "(c, i#is) |\<in>| vertices \<longleftrightarrow> c \<in> set conclusions \<and> i = plain_ant c \<and> is \<in> it_paths (it' c)"
   by (auto simp add: mem_vertices)
 
 lemma vertices_cases[consumes 1, case_names None Some]:
   assumes "v |\<in>| vertices"
   obtains c where "c \<in> set conclusions" and "v = (c, [])"
-      |   c "is" where "c \<in> set conclusions" and "is \<in> it_paths (it c)" and "v = (c, plain_ant c#is)"
+      |   c "is" where "c \<in> set conclusions" and "is \<in> it_paths (it' c)" and "v = (c, plain_ant c#is)"
 using assms by (cases v; rename_tac "is"; case_tac "is"; auto)
 
 lemma vertices_induct[consumes 1, case_names None Some]:
   assumes "v |\<in>| vertices"
   assumes "\<And> c. c \<in> set conclusions \<Longrightarrow> P (c, [])"
-  assumes "\<And> c is . c \<in> set conclusions \<Longrightarrow> is \<in> it_paths (it c) \<Longrightarrow> P (c, plain_ant c#is)"
+  assumes "\<And> c is . c \<in> set conclusions \<Longrightarrow> is \<in> it_paths (it' c) \<Longrightarrow> P (c, plain_ant c#is)"
   shows "P v"
 using assms by (cases v; rename_tac "is"; case_tac "is"; auto)
 
+lemma global_iwf_it:
+  assumes "c \<in> set conclusions"
+  shows "global_iwf (it' c) (fst (root (ts (to_form c))))"
+  using assms by (auto intro!: iwf_to_it globalized ts_finite ts_wf)
 
-definition preform_of_closed_form :: "'form \<Rightarrow> 'preform" where
-  "preform_of_closed_form f = (SOME pf. subst undefined (freshen undefined pf) = f)"
+text {* Start building the graph *}
 
 fun nodeOf :: "('preform, 'var) vertex \<Rightarrow> ('preform, 'rule) graph_node" where
   "nodeOf (pf, []) = Conclusion pf"
-| "nodeOf (pf, i#is) = iNodeOf (tree_at (it pf) is)"
+| "nodeOf (pf, i#is) = iNodeOf (tree_at (it' pf) is)"
 
 fun inst where
   "inst (c,[]) = undefined"
- |"inst (c, i#is) = iSubst (tree_at (it c) is)" 
+ |"inst (c, i#is) = iSubst (tree_at (it' c) is)" 
 
 
-lemma iNodeOf_outPorts:
-  "iwf' t ent \<Longrightarrow> x \<in> it_paths t \<Longrightarrow> outPorts (iNodeOf (tree_at t x)) = {||} \<Longrightarrow> False"
-  apply (induction arbitrary: x rule: iwf'.induct)
-  apply (case_tac x)
-  apply (auto elim!: it_paths_ConsE)
-  apply force
-  done
 
 lemma terminal_is_nil[simp]: "v |\<in>| vertices \<Longrightarrow> outPorts (nodeOf v) = {||} \<longleftrightarrow> snd v = []"
  apply (induction v rule: nodeOf.induct)
  apply auto
  apply (erule (1) iNodeOf_outPorts[rotated])
- apply (erule iwf'_it)
+ apply (erule global_iwf_it)
  done
 
-lemma iNodeOf_tree_at:
-  "iwf' t ent \<Longrightarrow> x \<in> it_paths t \<Longrightarrow> iNodeOf (tree_at t x) \<in> sset nodes"
-  apply (induction arbitrary: x rule: iwf'.induct)
-  apply (case_tac x)
-  apply (auto elim!: it_paths_ConsE)
-  apply force
-  done
 
 sublocale Vertex_Graph nodes inPorts outPorts vertices nodeOf.
 
 
 definition edge_from :: "'preform \<Rightarrow> ('preform, 'var) in_port list => (('preform, 'var) vertex \<times> ('preform,'var) out_port)" where 
-  "edge_from c is = ((c, plain_ant c # is),  Reg (iOutPort (tree_at (it c) is)))"
+  "edge_from c is = ((c, plain_ant c # is),  Reg (iOutPort (tree_at (it' c) is)))"
 
 lemma fst_edge_from[simp]: "fst (edge_from c is) = (c, plain_ant c # is)"
   by (simp add: edge_from_def)
@@ -458,188 +127,40 @@ definition edge_at :: "'preform \<Rightarrow> ('preform, 'var) in_port list => (
 lemma fst_edge_at[simp]: "fst (edge_at c i) = edge_from c i" by (simp add: edge_at_def)
 lemma snd_edge_at[simp]: "snd (edge_at c i) = edge_to c i" by (simp add: edge_at_def)
 
-inductive_set hyps_along for t "is" where
- "prefixeq (is'@[i]) is \<Longrightarrow>
-  hyps (iNodeOf (tree_at t is')) h = Some i \<Longrightarrow>
-  subst (iSubst  (tree_at t is')) (freshen (iAnnot (tree_at t is')) (labelsOut (iNodeOf (tree_at t is')) h)) \<in> hyps_along t is"
 
-lemma hyps_along_Nil[simp]: "hyps_along t [] = {}"
-  by (auto simp add: hyps_along.simps)
-
-lemma prefixeq_app_Cons_elim:
-  assumes "prefixeq (xs@[y]) (z#zs)"
-  obtains "xs = []" and "y = z"
-   | xs' where "xs = z#xs'" and "prefixeq (xs'@[y]) zs"
-using assms by (cases xs) auto
-
-lemma prefixeq_app_Cons_simp:
-  "prefixeq (xs@[y]) (z#zs) \<longleftrightarrow> (xs = [] \<and> y = z \<or> xs = z#tl xs \<and> prefixeq (tl xs@[y]) zs)"
- by (cases xs) auto
-
-lemma hyps_along_Cons:
-  assumes "i#is \<in> it_paths t"
-  shows "hyps_along t (i#is) =
-    (\<lambda>h. subst (iSubst t) (freshen (iAnnot t) (labelsOut (iNodeOf t) h))) ` fset (hyps_for (iNodeOf t) i)
-    \<union> hyps_along (the (iAnts t i)) is" (is "?S1 = ?S2 \<union> ?S3")
-proof-
-  from assms
-  obtain t' where "i |\<in>| inPorts (iNodeOf t)" and [simp]: "iAnts t i = Some t'" and "is \<in> it_paths t'"
-    by (auto elim: it_paths_ConsE)
-
-  show ?thesis
-  proof (rule; rule)
-    fix x
-    assume "x \<in> hyps_along t (i # is)"
-    then obtain is' i' h where
-      "prefixeq (is'@[i']) (i#is)"
-      and "hyps (iNodeOf (tree_at t is')) h = Some i'"
-      and [simp]: "x = subst (iSubst  (tree_at t is')) (freshen (iAnnot (tree_at t is')) (labelsOut (iNodeOf (tree_at t is')) h))"
-    by (auto elim: hyps_along.cases)
-    from this(1)
-    show "x \<in> ?S2 \<union> ?S3"
-    proof(cases rule: prefixeq_app_Cons_elim)
-      assume "is' = []" and "i' = i"
-      with `hyps (iNodeOf (tree_at t is')) h = Some i'`
-      have "x \<in> ?S2" by auto
-      thus ?thesis..
-    next
-      fix is''
-      assume [simp]: "is' = i # is''" and "prefixeq (is'' @ [i']) is"
-
-      from `hyps (iNodeOf (tree_at t is')) h = Some i'`
-      have "hyps (iNodeOf (tree_at t' is'')) h = Some i'" by simp
-
-      from hyps_along.intros[OF `prefixeq (is'' @ [i']) is` this]
-      have "subst (iSubst (tree_at t' is'')) (freshen (iAnnot (tree_at t' is'')) (labelsOut (iNodeOf (tree_at t' is'')) h))  \<in> hyps_along t' is".
-      hence "x \<in> ?S3" by simp
-      thus ?thesis..
-    qed
-  next
-    fix x
-    assume "x \<in> ?S2 \<union> ?S3"
-    thus "x \<in> ?S1"
-    proof
-      have "prefixeq ([]@[i]) (i#is)" by simp
-      
-      assume "x \<in> ?S2"
-      then obtain h where "h |\<in>| hyps_for (iNodeOf t) i"
-        and [simp]: "x = subst (iSubst t) (freshen (iAnnot t) (labelsOut (iNodeOf t) h))" by auto
-      from this(1)
-      have "hyps (iNodeOf (tree_at t [])) h = Some i" by simp
-      
-      from hyps_along.intros[OF `prefixeq ([]@[i]) (i#is)` this]
-      show "x \<in> hyps_along t (i # is)" by simp
-    next
-      assume "x \<in> ?S3"
-      thus "x \<in> ?S1"
-        apply (auto simp add: hyps_along.simps)
-        apply (rule_tac x = "i#is'" in exI)
-        apply auto
-        done
-    qed
-  qed
-qed
-      
-lemma hyps_exist:
+lemma pre_hyps_exist:
   assumes "c \<in> set conclusions"
-  assumes "is \<in> it_paths (it c)"
-  assumes "tree_at (it c) is = (HNode i s)"
-  shows "subst s (freshen i anyP) \<in> hyps_along (it c) is"
+  assumes "is \<in> it_paths (pre_it c)"
+  assumes "tree_at (pre_it c) is = (HNode i s)"
+  shows "subst s (freshen i anyP) \<in> hyps_along (pre_it c) is"
 proof-
   from assms(1)
-  have "iwf' (it c) (fst (root (ts (to_form c))))" by (rule iwf'_it)
-  note this assms(2,3)
-  hence "subst s (freshen i anyP) \<in> hyps_along (it c) is 
-     \<or> subst s (freshen i anyP) |\<in>| fst (fst (root (ts (to_form c))))
-       \<and> subst s (freshen i anyP) |\<notin>| ass_forms"
-  proof(induction arbitrary: "is" rule: iwf'.induct)
-    case (iwf' n p ants s' i' \<Gamma> c "is")
-   
-    show ?case
-    proof(cases "is")
-      case Nil
-      with `tree_at (INode n p i' s' ants) is = HNode i s`
-      show ?thesis by auto
-    next
-      case (Cons ip "is'")
-      with `is \<in> it_paths (INode n p i' s' ants)`
-      obtain it where "ip |\<in>| inPorts n" and [simp]: "ants ip = Some it" and "is' \<in> it_paths it"
-        by (auto elim: it_paths_ConsE)
-
-      let ?\<Gamma>' = "(\<lambda>h. subst s' (freshen i' (labelsOut n h))) |`| hyps_for n ip"
-      
-      from `tree_at (INode n p i' s' ants) is = HNode i s`
-      have "tree_at it is' = HNode i s" using Cons `ants ip = Some it` by simp
-
-      from  iwf'.IH[OF `ip |\<in>| _`] `ants ip = Some it` `is' \<in> it_paths it` this
-      have  "subst s (freshen i anyP) \<in> hyps_along it is'
-        \<or> subst s (freshen i anyP) |\<in>| ?\<Gamma>' |\<union>| \<Gamma> \<and> subst s (freshen i anyP) |\<notin>| ass_forms"
-        by auto
-      moreover
-      from  `is \<in> it_paths (INode n p i' s' ants)`
-      have "hyps_along (INode n p i' s' ants) is = fset ?\<Gamma>' \<union> hyps_along it is'"
-        using `is = _` by (simp add: hyps_along_Cons)
-      ultimately
-      show ?thesis by auto
-    qed
-  next
-    case (iwf'H c  \<Gamma> s' i' "is")
-    hence [simp]: "is = []" "i' = i" "s' = s" by simp_all
-    from `c = subst s' (freshen i' anyP)` `c |\<in>| \<Gamma>` `c |\<notin>| ass_forms`
-    show ?case by simp
-  qed
+  have "local_iwf (pre_it c) (fst (root (ts (to_form c))))" by (rule iwf_pre_it)
+  moreover
+  note assms(2,3)
   moreover
   have "fst (fst (root (ts (to_form c)))) |\<subseteq>| ass_forms"
     by (simp add: assms(1) ts_context)
   ultimately
-  show ?thesis by blast
+  show ?thesis by (rule iwf_hyps_exist)
 qed
 
-
-definition hyp_port_for' where
-  "hyp_port_for' t is f = (SOME x.
-   (case x of (is', i, h) \<Rightarrow> 
-      prefixeq (is' @ [i]) is \<and>
-      hyps (iNodeOf (tree_at t is')) h = Some i \<and>
-      f = subst (iSubst  (tree_at t is')) (freshen (iAnnot (tree_at t is')) (labelsOut (iNodeOf (tree_at t is')) h))
-   ))"
-
-lemma hyp_port_for_spec':
-  assumes "f \<in> hyps_along t is"
-  shows "(case hyp_port_for' t is f of (is', i, h) \<Rightarrow> 
-      prefixeq (is' @ [i]) is \<and>
-      hyps (iNodeOf (tree_at t is')) h = Some i \<and>
-      f = subst (iSubst  (tree_at t is')) (freshen (iAnnot (tree_at t is')) (labelsOut (iNodeOf (tree_at t is')) h)))"
-using assms unfolding hyps_along.simps hyp_port_for'_def by -(rule someI_ex, blast)
-
-definition hyp_port_path_for where "hyp_port_path_for t is f = fst (hyp_port_for' t is f)"
-definition hyp_port_i_for where "hyp_port_i_for t is f = fst (snd (hyp_port_for' t is f))"
-definition hyp_port_h_for where "hyp_port_h_for t is f = snd (snd (hyp_port_for' t is f))"
-
-lemma hyp_port_prefixeq:
-  assumes "f \<in> hyps_along t is"
-  shows "prefixeq (hyp_port_path_for t is f@[hyp_port_i_for t is f]) is"
-using hyp_port_for_spec'[OF assms] unfolding hyp_port_path_for_def hyp_port_i_for_def by auto
-
-lemma hyp_port_prefix:
-  assumes "f \<in> hyps_along t is"
-  shows "prefix (hyp_port_path_for t is f) is"
-using hyp_port_prefixeq[OF assms] by (simp add: prefixI' prefix_order.dual_order.strict_trans1)
-
-lemma hyp_port_hyps:
-  assumes "f \<in> hyps_along t is"
-  shows "hyps (iNodeOf (tree_at t (hyp_port_path_for t is f))) (hyp_port_h_for t is f) = Some (hyp_port_i_for t is f)"
-using hyp_port_for_spec'[OF assms] unfolding hyp_port_path_for_def hyp_port_i_for_def hyp_port_h_for_def by auto
-
-lemma hyp_port_outPort:
-  assumes "f \<in> hyps_along t is"
-  shows "(hyp_port_h_for t is f) |\<in>| outPorts (iNodeOf (tree_at t (hyp_port_path_for t is f)))"
-using hyps_correct[OF hyp_port_hyps[OF assms]]..
-
-lemma hyp_port_eq:
-  assumes "f \<in> hyps_along t is"
-  shows "f = subst (iSubst (tree_at t (hyp_port_path_for t is f))) (freshen (iAnnot (tree_at t (hyp_port_path_for t is f))) (labelsOut (iNodeOf (tree_at t (hyp_port_path_for t is f))) (hyp_port_h_for t is f)))"
-using hyp_port_for_spec'[OF assms] unfolding hyp_port_path_for_def hyp_port_i_for_def hyp_port_h_for_def by auto
+lemma hyps_exist':
+  assumes "c \<in> set conclusions"
+  assumes "is \<in> it_paths (it' c)"
+  assumes "tree_at (it' c) is = (HNode i s)"
+  shows "subst s (freshen i anyP) \<in> hyps_along (it' c) is"
+proof-
+  from assms(1)
+  have "global_iwf (it' c) (fst (root (ts (to_form c))))" by (rule global_iwf_it)
+  moreover
+  note assms(2,3)
+  moreover
+  have "fst (fst (root (ts (to_form c)))) |\<subseteq>| ass_forms"
+    by (simp add: assms(1) ts_context)
+  ultimately
+  show ?thesis by (rule iwf_hyps_exist)
+qed
 
 
 
@@ -648,7 +169,7 @@ definition hyp_edge_to where
 
 definition hyp_edge_from where
   "hyp_edge_from c is n s = 
-    ((c, plain_ant c # hyp_port_path_for (it c) is (subst s (freshen n anyP))), hyp_port_h_for (it c) is (subst s (freshen n anyP)))"
+    ((c, plain_ant c # hyp_port_path_for (it' c) is (subst s (freshen n anyP))), hyp_port_h_for (it' c) is (subst s (freshen n anyP)))"
 
 definition hyp_edge_at where
   "hyp_edge_at c is n s = (hyp_edge_from c is n s, hyp_edge_to c is)"
@@ -659,48 +180,37 @@ lemma snd_hyp_edge_at[simp]:
   "snd (hyp_edge_at c is n s) = hyp_edge_to c is" by (simp add:hyp_edge_at_def)
 
 inductive_set edges where
-  regular_edge: "c \<in> set conclusions \<Longrightarrow> is \<in> it_paths (it c) \<Longrightarrow> edge_at c is \<in> edges"
-  | hyp_edge: "c \<in> set conclusions \<Longrightarrow> is \<in> it_paths (it c) \<Longrightarrow> tree_at (it c) is = HNode n s \<Longrightarrow> hyp_edge_at c is n s \<in> edges"
+  regular_edge: "c \<in> set conclusions \<Longrightarrow> is \<in> it_paths (it' c) \<Longrightarrow> edge_at c is \<in> edges"
+  | hyp_edge: "c \<in> set conclusions \<Longrightarrow> is \<in> it_paths (it' c) \<Longrightarrow> tree_at (it' c) is = HNode n s \<Longrightarrow> hyp_edge_at c is n s \<in> edges"
 
 sublocale Pre_Port_Graph nodes inPorts outPorts vertices nodeOf edges.
 
-lemma iwf'_outPort: 
-  assumes "iwf' t ent"
-  assumes "x \<in> it_paths t"
-  shows "Reg (iOutPort (tree_at t x)) |\<in>| outPorts (iNodeOf (tree_at t x))"
-using assms
-  apply (induction arbitrary: x rule: iwf'.induct)
-  apply (case_tac x)
-  apply (auto elim!: it_paths_ConsE)
-  apply force
-  done
-
 lemma edge_from_valid_out_port:
-  assumes "p \<in> it_paths (it c)"
+  assumes "p \<in> it_paths (it' c)"
   assumes "c \<in> set conclusions"
   shows "valid_out_port (edge_from c p)"
 using assms
-by (auto simp add: edge_from_def intro: iwf'_outPort iwf'_it)
+by (auto simp add: edge_from_def intro: iwf_outPort global_iwf_it)
 
 lemma edge_to_valid_in_port:
-  assumes "p \<in> it_paths (it c)"
+  assumes "p \<in> it_paths (it' c)"
   assumes "c \<in> set conclusions"
   shows "valid_in_port (edge_to c p)"
 using assms
 by (auto simp add: edge_to_def split: list.split elim!: it_path_SnocE)
 
 lemma hyp_edge_from_valid_out_port:
-  assumes "is \<in> it_paths (it c)"
+  assumes "is \<in> it_paths (it' c)"
   assumes "c \<in> set conclusions"
-  assumes "tree_at (it c) is = HNode n s"
+  assumes "tree_at (it' c) is = HNode n s"
   shows "valid_out_port (hyp_edge_from c is n s)"
 using assms
-by(auto simp add: hyp_edge_from_def intro: hyp_port_outPort it_paths_prefix hyp_port_prefix  hyps_exist)
+by(auto simp add: hyp_edge_from_def intro: hyp_port_outPort it_paths_prefix hyp_port_prefix  hyps_exist')
 
 lemma hyp_edge_to_valid_in_port:
-  assumes "is \<in> it_paths (it c)"
+  assumes "is \<in> it_paths (it' c)"
   assumes "c \<in> set conclusions"
-  assumes "tree_at (it c) is = HNode n s"
+  assumes "tree_at (it' c) is = HNode n s"
   shows "valid_in_port (hyp_edge_to c is)"
 using assms by (auto simp add: hyp_edge_to_def)
 
@@ -708,7 +218,7 @@ using assms by (auto simp add: hyp_edge_to_def)
 
 inductive scope' where
   "c \<in> set conclusions \<Longrightarrow>
-   is' \<in> (op # (plain_ant c)) ` it_paths (it c) \<Longrightarrow>
+   is' \<in> (op # (plain_ant c)) ` it_paths (it' c) \<Longrightarrow>
    prefixeq (is@[i]) is' \<Longrightarrow> 
    scope' (c, is) i (c, is')"
 
@@ -751,7 +261,7 @@ lemma terminal_path_from_Snoc[simp]:
 
 lemma path_terminal_path_from:
   "c \<in> set conclusions \<Longrightarrow>
-  is \<in> it_paths (it c) \<Longrightarrow>
+  is \<in> it_paths (it' c) \<Longrightarrow>
   path (c, plain_ant c # is) (c, []) (terminal_path_from c is)"
 by (induction "is" rule: rev_induct)
    (auto simp add: path_cons_simp intro!: regular_edge elim: it_path_SnocE)
@@ -768,10 +278,10 @@ proof(cases rule: edges.cases[consumes 1, case_names Reg Hyp])
   thus thesis by (rule that)
 next
   case (Hyp c "is" n s)
-  hence "a = aa" and "prefixeq (b@[hyp_port_i_for (it c) is (subst s (freshen n anyP))]) bb" and
-    "hyps (nodeOf (a, b)) ba = Some (hyp_port_i_for (it c) is (subst s (freshen n anyP)))"
+  hence "a = aa" and "prefixeq (b@[hyp_port_i_for (it' c) is (subst s (freshen n anyP))]) bb" and
+    "hyps (nodeOf (a, b)) ba = Some (hyp_port_i_for (it' c) is (subst s (freshen n anyP)))"
   by (auto simp add: edge_at_def edge_from_def edge_to_def hyp_edge_at_def hyp_edge_to_def hyp_edge_from_def
-      intro: hyp_port_prefixeq hyps_exist hyp_port_hyps)
+      intro: hyp_port_prefixeq hyps_exist' hyp_port_hyps)
   thus thesis by (rule that)
 qed
 
@@ -799,7 +309,7 @@ proof
   next
     case (Some c "is")
 
-    from `c \<in> set conclusions` `is \<in> it_paths (it c)`
+    from `c \<in> set conclusions` `is \<in> it_paths (it' c)`
     have "path (c, plain_ant c # is) (c, []) (terminal_path_from c is)"
       by (rule path_terminal_path_from)
     moreover
@@ -818,14 +328,14 @@ proof
       with `(v',p') = edge_to c is'`
       have "v' = (c, [])" and "p' = plain_ant c"
         by (auto simp add: edge_to_def)
-      with `c \<in> set conclusions` `is \<in> it_paths (it c)`
+      with `c \<in> set conclusions` `is \<in> it_paths (it' c)`
       show ?thesis  by (auto intro!: scope'.intros)
     next
       case (snoc is'' i)
       with `(v',p') = edge_to c is'`
       have "v' = (c, plain_ant c # is'')" and "p' = i"
         by (auto simp add: edge_to_def)
-      with `c \<in> set conclusions` `is \<in> it_paths (it c)` `prefixeq is' is`[unfolded snoc]
+      with `c \<in> set conclusions` `is \<in> it_paths (it' c)` `prefixeq is' is`[unfolded snoc]
       show ?thesis
         by (auto intro!: scope'.intros)
     qed
@@ -835,7 +345,7 @@ next
   assume "scope' v' p' v"
   then obtain c is' "is" where
     "v' = (c, is')" and "v = (c, is)" and "c \<in> set conclusions" and
-    "is \<in> op # (plain_ant c) ` it_paths (it c)" and  "prefixeq (is' @ [p']) is"
+    "is \<in> op # (plain_ant c) ` it_paths (it' c)" and  "prefixeq (is' @ [p']) is"
     by (auto simp add: scope'.simps)
 
   from `scope' v' p' v`
@@ -858,7 +368,7 @@ sublocale Port_Graph nodes inPorts outPorts vertices nodeOf edges
 proof
   show "nodeOf ` fset vertices \<subseteq> sset nodes"
     apply (auto simp add: fmember.rep_eq[symmetric] mem_vertices)
-    apply (auto simp add: stream.set_map dest: iNodeOf_tree_at[OF iwf'_it])
+    apply (auto simp add: stream.set_map dest: iNodeOf_tree_at[OF global_iwf_it])
     done
   next
 
@@ -880,6 +390,15 @@ lemma hyps_free_path_length:
 using assms by induction (auto elim!: edge_step )
 
 sublocale Instantiation inPorts outPorts nodeOf hyps fv ran_fv closed anyP nodes edges vertices labelsIn labelsOut pre_fv subst freshen inst..
+
+lemma fidx_iAnnot:
+  assumes "is \<in> it_paths (it c)"
+  shows "fidx vertices (c, plain_ant c # is) = iAnnot (tree_at (it c) is)"
+using assms
+apply(induction "is" arbitrary: c rule: it_paths_induct)
+apply simp
+find_theorems it
+oops
 
 sublocale Tasked_Proof_Graph freshen fv ran_fv closed anyP subst pre_fv antecedent consequent fresh_vars rules assumptions conclusions
   vertices nodeOf edges inst
@@ -920,7 +439,7 @@ proof
       with `valid_in_port ((c, cis), p)`
       have [simp]: "p = plain_ant c" by simp
 
-      have "[] \<in> it_paths (it c)" by simp
+      have "[] \<in> it_paths (it' c)" by simp
       with `c \<in> set conclusions`
       have "edge_at c [] \<in> edges" by (rule regular_edge)
       moreover
@@ -931,14 +450,14 @@ proof
     next
       case (Cons c' "is")
       with `valid_in_port ((c, cis), p)`
-      have [simp]: "c' = plain_ant c" and "is \<in> it_paths (it c)"
-        and "p |\<in>| inPorts (iNodeOf (tree_at (it c) is))" by auto
+      have [simp]: "c' = plain_ant c" and "is \<in> it_paths (it' c)"
+        and "p |\<in>| inPorts (iNodeOf (tree_at (it' c) is))" by auto
       show ?thesis
-      proof (cases "tree_at (it c) is")
+      proof (cases "tree_at (it' c) is")
         case INode
-        hence "\<not> isHNode (tree_at (it c) is)" by simp
-        from iwf'_it[OF `c \<in> set conclusions`] `is \<in> it_paths (it c)` this `p |\<in>| inPorts (iNodeOf (tree_at (it c) is))`
-        have "is@[p] \<in> it_paths (it c)" by (rule it_path_SnocI)
+        hence "\<not> isHNode (tree_at (it' c) is)" by simp
+        from global_iwf_it[OF `c \<in> set conclusions`] `is \<in> it_paths (it' c)` this `p |\<in>| inPorts (iNodeOf (tree_at (it' c) is))`
+        have "is@[p] \<in> it_paths (it' c)" by (rule it_path_SnocI)
         from `c \<in> set conclusions` this
         have "edge_at c (is@[p]) \<in> edges" by (rule regular_edge)
         moreover
@@ -948,10 +467,10 @@ proof
         show ?thesis by (auto simp add: Cons simp del: snd_edge_at)
       next
         case (HNode n s)
-        from `c \<in> set conclusions` `is \<in> it_paths (it c)`  this
+        from `c \<in> set conclusions` `is \<in> it_paths (it' c)`  this
         have "hyp_edge_at c is n s \<in> edges"..
         moreover
-        from HNode `p |\<in>| inPorts (iNodeOf (tree_at (it c) is))`
+        from HNode `p |\<in>| inPorts (iNodeOf (tree_at (it' c) is))`
         have [simp]: "p = plain_ant anyP" by simp
 
         have "snd (hyp_edge_at c is n s) = ((c, plain_ant c # is), p)"
@@ -985,17 +504,25 @@ proof
   fix v\<^sub>1 p\<^sub>1 v\<^sub>2 p\<^sub>2
   assume "((v\<^sub>1, p\<^sub>1), (v\<^sub>2, p\<^sub>2)) \<in> edges"
   thus "labelAtOut v\<^sub>1 p\<^sub>1 = labelAtIn v\<^sub>2 p\<^sub>2"
-  proof(cases)
+  proof(cases rule:edges.cases)
     case (regular_edge c "is")
+   
+    from `((v\<^sub>1, p\<^sub>1), v\<^sub>2, p\<^sub>2) = edge_at c is`
+    have "(v\<^sub>1,p\<^sub>1) = edge_from c is" using fst_edge_at by (metis fst_conv)
+    hence "v\<^sub>1 = (c, plain_ant c # is)" by (simp add: edge_from_def)
+    moreover have "fidx vertices (c, plain_ant c # is) = iAnnot (tree_at (it' c) is)" sorry
+    ultimately have fidx: "fidx vertices v\<^sub>1 = iAnnot (tree_at (it' c) is)" by simp
+
     show ?thesis
     proof(cases "is" rule:rev_cases)
       case Nil
-      let "?t'" = "it c"
+      let "?t'" = "it' c"
       have "labelAtOut v\<^sub>1 p\<^sub>1 = subst (iSubst ?t') (freshen (fidx vertices v\<^sub>1) (iOutPort ?t'))"
         using regular_edge Nil by (simp add: labelAtOut_def edge_at_def edge_from_def)
-      also have "fidx vertices v\<^sub>1 = iAnnot ?t'" sorry
+      also have "fidx vertices v\<^sub>1 = iAnnot ?t'"
+        using fidx Nil by simp
       also have "subst (iSubst ?t') (freshen (iAnnot ?t') (iOutPort ?t')) = snd (fst (tree.root (ts (to_form c))))"
-        unfolding iwf'_subst_freshen_outPort[OF iwf'_it[OF `c \<in> set conclusions`]]..
+        unfolding iwf_subst_freshen_outPort[OF global_iwf_it[OF `c \<in> set conclusions`]]..
       also have "\<dots> = to_form c" using `c \<in> set conclusions` by (simp add: ts_conc)
       also have "\<dots> = subst undefined (freshen (fidx vertices (c, [])) c)"
         using  `c \<in> set conclusions` by (simp add: closed_eq[OF conclusions_closed])
@@ -1004,13 +531,15 @@ proof
       finally show ?thesis.
     next
       case (snoc is' i)
-      let "?t1" = "tree_at (it c) (is'@[i])"
-      let "?t2" = "tree_at (it c) is'"
+      let "?t1" = "tree_at (it' c) (is'@[i])"
+      let "?t2" = "tree_at (it' c) is'"
       have "labelAtOut v\<^sub>1 p\<^sub>1 = subst (iSubst ?t1) (freshen (fidx vertices v\<^sub>1) (iOutPort ?t1))"
         using regular_edge snoc by (simp add: labelAtOut_def edge_at_def edge_from_def)
-      also have "fidx vertices v\<^sub>1 = iAnnot ?t1" sorry
+      also have "fidx vertices v\<^sub>1 = iAnnot ?t1" using fidx snoc by simp
       also have "subst (iSubst ?t1) (freshen (iAnnot ?t1) (iOutPort ?t1)) = subst (iSubst ?t2) (freshen (iAnnot ?t2) (a_conc i))"
-        by (rule iwf'_edge_match[OF iwf'_it[OF `c \<in> set conclusions`] `is \<in> it_paths (it c)`[unfolded snoc]])
+        apply (rule iwf_edge_match[OF global_iwf_it[OF `c \<in> set conclusions`]])
+        apply (simp add: `is \<in> it_paths (it' c)`[unfolded snoc])
+        done
       also have "iAnnot ?t2 = (fidx vertices (c, plain_ant c # is'))" sorry
       also have "subst (iSubst ?t2) (freshen (fidx vertices (c, plain_ant c # is')) (a_conc i)) = labelAtIn v\<^sub>2 p\<^sub>2"
         using regular_edge snoc by (simp add: labelAtIn_def edge_at_def)
@@ -1019,20 +548,21 @@ proof
   next
     case (hyp_edge c "is" n s)
     let ?f = "subst s (freshen n anyP)"
-    let ?h = "hyp_port_h_for (it c) is ?f"
-    let ?his = "hyp_port_path_for (it c) is ?f"
-    let "?t1" = "tree_at (it c) ?his"
-    let "?t2" = "tree_at (it c) is"
+    let ?h = "hyp_port_h_for (it' c) is ?f"
+    let ?his = "hyp_port_path_for (it' c) is ?f"
+    let "?t1" = "tree_at (it' c) ?his"
+    let "?t2" = "tree_at (it' c) is"
 
-    from `c \<in> set conclusions` `is \<in> it_paths (it c)` `tree_at (it c) is = HNode n s`
-    have "?f \<in> hyps_along (it c) is"
-      by (rule hyps_exist)
+    have fidx: "fidx vertices v\<^sub>1 = iAnnot (tree_at (it' c) is)" sorry
+
+    from `c \<in> set conclusions` `is \<in> it_paths (it' c)` `tree_at (it' c) is = HNode n s`
+    have "?f \<in> hyps_along (it' c) is"
+      by (rule hyps_exist')
 
     have "labelAtOut v\<^sub>1 p\<^sub>1 = subst (iSubst ?t1) (freshen (fidx vertices v\<^sub>1) (labelsOut (iNodeOf ?t1) ?h))"
       using hyp_edge by (simp add: hyp_edge_at_def hyp_edge_from_def labelAtOut_def)
-    also have "\<dots> = subst (iSubst ?t1) (freshen (iAnnot ?t1) (labelsOut (iNodeOf ?t1) ?h))"
-      sorry
-    also have "\<dots> = ?f" using `?f \<in> hyps_along (it c) is` by (rule local.hyp_port_eq[symmetric])
+    also have "\<dots> = subst (iSubst ?t1) (freshen (iAnnot ?t1) (labelsOut (iNodeOf ?t1) ?h))" sorry
+    also have "\<dots> = ?f" using `?f \<in> hyps_along (it' c) is` by (rule local.hyp_port_eq[symmetric])
     also have "\<dots> = subst (iSubst ?t2) (freshen (iAnnot ?t2) anyP)"
       using hyp_edge by simp
     also have "iAnnot ?t2 = (fidx vertices (c, plain_ant c # is))" sorry
