Incredible_Trees.thy
@@ -1,0 +1,581 @@
+theory Incredible_Trees
+imports Natural_Deduction Incredible_Deduction
+begin
+
+lemma prefixeq_snocD: "prefixeq (xs@[x]) ys \<Longrightarrow> prefix xs ys"
+  by (simp add: prefixI' prefix_order.dual_order.strict_trans1)
+
+lemma image_eq_to_f:
+  assumes  "f1 ` S1 = f2 ` S2"
+  obtains f where "\<And> x. x \<in> S2 \<Longrightarrow> f x \<in> S1 \<and> f1 (f x) = f2 x"
+proof (atomize_elim)
+  from assms
+  have "\<forall>x. x \<in> S2 \<longrightarrow> (\<exists> y. y \<in> S1 \<and> f1 y = f2 x)" by (metis image_iff)
+  thus "\<exists>f. \<forall>x. x \<in> S2 \<longrightarrow> f x \<in> S1 \<and> f1 (f x) = f2 x" by metis
+qed
+
+context includes fset.lifting
+begin
+lemma fimage_eq_to_f:
+  assumes  "f1 |`| S1 = f2 |`| S2"
+  obtains f where "\<And> x. x |\<in>| S2 \<Longrightarrow> f x |\<in>| S1 \<and> f1 (f x) = f2 x"
+using assms apply transfer using image_eq_to_f by metis
+end
+
+
+section {* Elaborated tree (annotation and substitution) *}
+
+text {*
+Tree-shape, but incredible-graph-like content (port names, explicit annotation and substitution)
+*}
+
+datatype ('preform,'rule,'subst,'var)  itree =
+    INode (iNodeOf': "('preform, 'rule) graph_node")
+          (iOutPort': "'preform reg_out_port")
+          (iAnnot: "nat")
+          (iSubst: "'subst")
+          (iAnts': "('preform, 'var) in_port \<rightharpoonup> ('preform,'rule,'subst,'var) itree")
+  | HNode (iAnnot: "nat")
+          (iSubst: "'subst")
+
+fun iAnts where
+   "iAnts (INode n p i s ants) = ants"
+ | "iAnts (HNode i s) = empty"
+
+fun iNodeOf where
+   "iNodeOf (INode n p i s ants) = n"
+ | "iNodeOf (HNode i s) = Helper"
+
+context Abstract_Formulas
+begin
+fun iOutPort where
+   "iOutPort (INode n p i s ants) = p"
+ | "iOutPort (HNode i s) = anyP"
+end
+
+type_synonym ('preform, 'rule, 'subst, 'form) fresh_check = "('preform, 'rule) graph_node \<Rightarrow> nat \<Rightarrow> 'subst \<Rightarrow> 'form entailment \<Rightarrow> bool"
+
+context  Abstract_Task
+begin
+
+  inductive iwf :: "('preform, 'rule, 'subst, 'form) fresh_check \<Rightarrow> ('preform,'rule,'subst,'var) itree \<Rightarrow> 'form entailment \<Rightarrow> bool"
+    for fc
+    where
+    iwf: "\<lbrakk>
+       n \<in> sset nodes;
+       Reg p |\<in>| outPorts n;
+       \<And> ip. ip |\<in>| inPorts n \<Longrightarrow>
+          (\<exists> t. ants ip = Some t \<and>
+              iwf fc t ((\<lambda> h . subst s (freshen i (labelsOut n h))) |`| hyps_for n ip |\<union>| \<Gamma> \<turnstile> subst s (freshen i (labelsIn n ip))));
+       fc n i s (\<Gamma> \<turnstile> c);
+       c = subst s (freshen i (labelsOut n (Reg p :: (('preform, 'var) out_port))))
+      \<rbrakk> \<Longrightarrow> iwf fc (INode n p i s ants) (\<Gamma> \<turnstile> c)"  
+  | iwfH: "\<lbrakk>
+       c |\<notin>| ass_forms;
+       c |\<in>| \<Gamma>;
+       c = subst s (freshen i anyP)
+      \<rbrakk> \<Longrightarrow> iwf fc (HNode i s) (\<Gamma> \<turnstile> c)"  
+
+lemma iwf_subst_freshen_outPort:
+  "iwf lc ts ent \<Longrightarrow>
+  snd ent = subst (iSubst ts) (freshen (iAnnot ts) (iOutPort ts))"
+  by (auto elim: iwf.cases)
+
+
+
+  inductive local_fresh_check :: "('preform, 'rule, 'subst, 'form) fresh_check" where
+    "\<lbrakk>\<And> ip. ip |\<in>| inPorts n  \<Longrightarrow> f |\<in>| \<Gamma> \<Longrightarrow> freshenV i ` (local_vars n ip) \<inter> fv f = {};
+      \<And> ip. ip |\<in>| inPorts n  \<Longrightarrow> freshenV i ` (local_vars n ip) \<inter> ran_fv s = {}
+     \<rbrakk> \<Longrightarrow> local_fresh_check n i s (\<Gamma> \<turnstile> c)"
+
+  abbreviation "local_iwf \<equiv> iwf local_fresh_check"
+  
+  
+lemma build_local_iwf:
+  fixes t :: "('form entailment \<times> ('rule \<times> 'preform) NatRule) tree"
+  assumes "tfinite t"
+  assumes "wf t"
+  shows "\<exists> it. local_iwf it (fst (root t))"
+using assms
+proof(induction)
+  case (tfinite t)
+  from `wf t`
+  have "snd (root t) \<in> R" using wf.simps by blast
+
+  from `wf t`
+  have "eff (snd (root t)) (fst (root t)) ((fst \<circ> root) |`| cont t)" using wf.simps by blast
+
+  from `wf t`
+  have "\<And> t'. t' |\<in>| cont t \<Longrightarrow> wf t'" using wf.simps by blast
+  hence IH: "\<And> \<Gamma>' t'. t' |\<in>| cont t \<Longrightarrow> (\<exists>it'. local_iwf it' (fst (root t')))" using tfinite(2) by blast
+  then obtain its where its: "\<And> t'. t' |\<in>| cont t \<Longrightarrow> local_iwf (its t') (fst (root t'))" by metis
+
+  from `eff _ _ _`
+  show ?case               
+  proof(cases rule: eff.cases[case_names Axiom NatRule Cut])
+  case (Axiom con \<Gamma>)
+    show ?thesis
+    proof (cases "con |\<in>| ass_forms")
+      case True (* Global assumption *)
+      then obtain c :: "'preform" where
+        "c \<in> set assumptions" and [simp]: "subst undefined (freshen undefined c) = con"
+        by (auto simp add:  ass_forms_def)
+
+      let "?it" = "INode (Assumption c) c undefined undefined empty ::  ('preform, 'rule, 'subst, 'var) itree"
+
+      from `c \<in> set assumptions`
+      have "local_iwf ?it (\<Gamma> \<turnstile> con)" by (auto intro!: iwf local_fresh_check.intros)
+      thus ?thesis unfolding Axiom..
+    next
+      case False
+      obtain s where [simp]: "subst s (freshen undefined anyP) = con" by atomize_elim (rule anyP_is_any)
+  
+      let "?it" = "HNode undefined s ::  ('preform, 'rule, 'subst, 'var) itree"
+  
+      from  `con |\<in>| \<Gamma>` False
+      have "local_iwf ?it (\<Gamma> \<turnstile> con)" by (auto intro: iwfH)
+      thus ?thesis unfolding Axiom..
+    qed
+  next
+  case (NatRule rule c ants \<Gamma> i s)
+    from `natEff_Inst rule c ants`
+    have "snd rule = c"  and [simp]: "f_antecedent (fst rule) = ants" and "c \<in> set (consequent (fst rule))"
+      by (auto simp add: natEff_Inst.simps)  
+
+    from `(fst \<circ> root) |\`| cont t = (\<lambda>ant. (\<lambda>p. subst s (freshen i p)) |\`| a_hyps ant |\<union>| \<Gamma> \<turnstile> subst s (freshen i (a_conc ant))) |\`| ants`
+    obtain to_t where "\<And> ant. ant |\<in>| ants \<Longrightarrow> to_t ant |\<in>| cont t \<and> (fst \<circ> root) (to_t ant) = ((\<lambda>p. subst s (freshen i p)) |`| a_hyps ant |\<union>| \<Gamma> \<turnstile> subst s (freshen i (a_conc ant)))"
+      by (rule fimage_eq_to_f) (rule that)
+    hence to_t_in_cont: "\<And> ant. ant |\<in>| ants \<Longrightarrow> to_t ant |\<in>| cont t"
+      and to_t_root: "\<And> ant. ant |\<in>| ants \<Longrightarrow>  fst (root (to_t ant)) = ((\<lambda>p. subst s (freshen i p)) |`| a_hyps ant |\<union>| \<Gamma> \<turnstile> subst s (freshen i (a_conc ant)))"
+      by auto
+
+    let "?it" = "INode (Rule (fst rule)) c i s (\<lambda> ant. if ant |\<in>| ants then Some (its (to_t ant)) else None) ::  ('preform, 'rule, 'subst, 'var) itree"
+
+    from `snd (root t) \<in> R`
+    have "fst rule \<in> sset rules"
+      unfolding NatRule
+      by (auto simp add: stream.set_map n_rules_def no_empty_conclusions )
+    moreover
+    from `c \<in> set (consequent (fst rule))`
+    have "c |\<in>| f_consequent (fst rule)" by (simp add: f_consequent_def)
+    moreover
+    { fix ant
+      assume "ant |\<in>| ants"
+      from its[OF to_t_in_cont[OF this]]
+      have "local_iwf (its (to_t ant)) (fst (root (to_t ant)))".
+      also have "fst (root (to_t ant)) =
+        ((\<lambda>h. subst s (freshen i (labelsOut (Rule (fst rule)) h))) |`| hyps_for (Rule (fst rule)) ant |\<union>| \<Gamma>
+         \<turnstile> subst s (freshen i (a_conc ant)))"
+        by (auto simp add: to_t_root `ant |\<in>| ants`)
+      finally
+      have "local_iwf (its (to_t ant))
+           ((\<lambda>h. subst s (freshen i (labelsOut (Rule (fst rule)) h))) |`| hyps_for (Rule (fst rule)) ant |\<union>|
+            \<Gamma>  \<turnstile> subst s (freshen i (a_conc ant)))".
+    }
+    moreover
+    note NatRule(5,6)
+    ultimately
+    have "local_iwf ?it ((\<Gamma> \<turnstile> subst s (freshen i c)))"
+      apply -
+      apply (intro iwf local_fresh_check.intros)
+      apply auto
+      apply blast
+      done
+    thus ?thesis unfolding NatRule..
+  next
+  case (Cut \<Gamma> con)
+    obtain s where [simp]: "subst s (freshen undefined anyP) = con" by atomize_elim (rule anyP_is_any)
+
+    from `(fst \<circ> root) |\`| cont t = {|\<Gamma> \<turnstile> con|}`
+    obtain t'  where "t' |\<in>| cont t" and [simp]: "fst (root t') = (\<Gamma> \<turnstile> con)"
+      by (cases "cont t") auto
+    
+    from `t' |\<in>| cont t` obtain "it'" where "local_iwf it' (\<Gamma> \<turnstile> con)" using IH by force
+
+    let "?it" = "INode Helper anyP undefined s (empty(plain_ant anyP \<mapsto> it')) ::  ('preform, 'rule, 'subst, 'var) itree"
+
+    from `local_iwf it' (\<Gamma> \<turnstile> con)`
+    have "local_iwf ?it (\<Gamma> \<turnstile> con)" by (auto intro!: iwf local_fresh_check.intros)
+    thus ?thesis unfolding Cut..
+  qed 
+qed
+
+definition to_it :: "('form entailment \<times> ('rule \<times> 'preform) NatRule) tree \<Rightarrow> ('preform,'rule,'subst,'var) itree" where
+  "to_it t = (SOME it. local_iwf it (fst (root t)))"
+
+lemma iwf_to_it:
+  assumes "tfinite t" and "wf t"
+  shows "local_iwf (to_it t) (fst (root t))"
+unfolding to_it_def using build_local_iwf[OF assms] by (rule someI2_ex)
+
+
+inductive it_pathsP :: "('preform,'rule,'subst,'var) itree \<Rightarrow> ('preform, 'var) in_port list \<Rightarrow> bool"  where
+   it_paths_Nil: "it_pathsP t []"
+ | it_paths_Cons: "i |\<in>| inPorts (iNodeOf t) \<Longrightarrow> iAnts t i = Some t' \<Longrightarrow> it_pathsP t' is \<Longrightarrow> it_pathsP t (i#is)"
+
+inductive_cases it_pathP_ConsE: "it_pathsP t (i#is)"
+
+definition it_paths:: "('preform,'rule,'subst,'var) itree \<Rightarrow> ('preform, 'var) in_port list set"  where
+  "it_paths t = Collect (it_pathsP t)"
+
+ lemma it_paths_eq [pred_set_conv]: "it_pathsP t = (\<lambda>x. x \<in> it_paths t)"
+   by(simp add: it_paths_def)
+
+ lemmas it_paths_intros [intro?] = it_pathsP.intros[to_set]
+ lemmas it_paths_induct [consumes 1, induct set: it_paths] = it_pathsP.induct[to_set]
+ lemmas it_paths_cases [consumes 1, cases set: it_paths] = it_pathsP.cases[to_set]
+ lemmas it_paths_ConsE = it_pathP_ConsE[to_set]
+ lemmas it_paths_simps = it_pathsP.simps[to_set]
+
+ lemma [simp]: "[] \<in> it_paths t" by (rule it_paths_intros)
+
+lemma it_paths_HNode[simp]: "it_paths (HNode i s) = {[]}"
+  by (auto elim: it_paths_cases)
+
+lemma it_paths_Union: "it_paths t \<subseteq> insert [] (Union (fset ((\<lambda> i. case iAnts t i of Some t \<Rightarrow> (op # i) ` it_paths t | None \<Rightarrow> {}) |`| (inPorts (iNodeOf t)))))"
+  apply (rule)
+  apply (subst (asm) it_paths_simps)
+  apply (fastforce split: prod.split simp add: fmember.rep_eq)
+  done
+
+lemma finite_it_paths[simp]: "finite (it_paths t)"
+  by (induction t) (rule finite_subset[OF it_paths_Union], fastforce split: option.split intro: range_eqI)+
+end
+
+fun tree_at :: "('preform,'rule,'subst,'var) itree \<Rightarrow> ('preform, 'var) in_port list \<Rightarrow> ('preform,'rule,'subst,'var) itree" where
+  "tree_at t [] = t"
+| "tree_at t (i#is) = tree_at (the (iAnts t i)) is"
+
+context Abstract_Task
+begin
+lemma it_path_SnocE[elim_format]:
+  assumes "is @ [i] \<in> it_paths t"
+  shows "is \<in> it_paths t \<and> i |\<in>| inPorts (iNodeOf (tree_at t is))"
+using assms
+by (induction "is" arbitrary: t)(auto intro!: it_paths_intros elim!: it_paths_ConsE)
+
+fun isHNode where
+  "isHNode (HNode _ _) = True"
+ |"isHNode _ = False"
+
+
+lemma it_paths_prefix:
+  assumes "is \<in> it_paths t"
+  assumes "prefix is' is"
+  shows "is' \<in> it_paths t"
+proof-
+  from assms(2)
+  obtain is'' where "is = is' @ is''" using prefixE' by blast
+  from assms(1)[unfolded this]
+  show ?thesis
+    by(induction is' arbitrary: t) (auto elim!: it_paths_ConsE intro!: it_paths_intros)
+qed
+end
+
+
+type_synonym ('preform, 'var) vertex = "('preform \<times> ('preform, 'var) in_port list)"
+type_synonym ('preform, 'var) edge'' = "(('preform, 'var) vertex, 'preform, 'var) edge'"
+
+context Abstract_Task
+begin
+lemma it_path_SnocI:
+  assumes "iwf fc t ant"
+  assumes "is \<in> it_paths t" 
+  assumes "\<not> isHNode (tree_at t is)"
+  assumes "i |\<in>| inPorts (iNodeOf (tree_at t is))"
+  shows "is @ [i] \<in> it_paths t"
+  using assms
+  apply (induction arbitrary: "is" i)
+  apply auto
+  apply (case_tac "is")
+  apply (force intro: it_paths_intros elim!: it_paths_ConsE)+
+  done
+
+lemma iwf_edge_match:
+  assumes "iwf fc t ent"
+  assumes "is@[i] \<in> it_paths t"
+  shows "subst (iSubst (tree_at t (is@[i]))) (freshen (iAnnot (tree_at t (is@[i]))) (iOutPort (tree_at t (is@[i]))))
+     = subst (iSubst (tree_at t is)) (freshen (iAnnot (tree_at t is)) (a_conc i))"
+  using assms
+  apply (induction arbitrary: "is" i)
+  apply (case_tac "is")
+  apply (force elim!: it_paths_ConsE intro: trans[OF iwf_subst_freshen_outPort[symmetric]])+
+  done
+
+end
+
+context Abstract_Task
+begin
+
+abbreviation to_form :: "'preform \<Rightarrow> 'form" where
+  "to_form pf \<equiv> subst undefined (freshen undefined pf)"
+
+lemma to_form_conc_forms[simp]: "to_form a |\<in>| conc_forms \<longleftrightarrow> a \<in> set conclusions"
+proof
+  assume "a \<in> set conclusions"
+  thus "to_form a |\<in>| conc_forms" by (rule subst_freshen_in_conc_formsI)
+next
+  assume "to_form a |\<in>| conc_forms"
+  then obtain a' where "a' \<in> set conclusions" and "to_form a = to_form a'"
+    by (auto simp add: conc_forms_def)
+  thus "a \<in> set conclusions" using conclusions_closed closed_eq by metis
+qed
+
+definition preform_of_closed_form :: "'form \<Rightarrow> 'preform" where
+  "preform_of_closed_form f = (SOME pf. subst undefined (freshen undefined pf) = f)"
+
+
+lemma iNodeOf_outPorts:
+  "iwf fc t ent \<Longrightarrow> x \<in> it_paths t \<Longrightarrow> outPorts (iNodeOf (tree_at t x)) = {||} \<Longrightarrow> False"
+  apply (induction arbitrary: x rule: iwf.induct)
+  apply (case_tac x)
+  apply (auto elim!: it_paths_ConsE)
+  apply force
+  done
+
+lemma iNodeOf_tree_at:
+  "iwf fc t ent \<Longrightarrow> x \<in> it_paths t \<Longrightarrow> iNodeOf (tree_at t x) \<in> sset nodes"
+  apply (induction arbitrary: x rule: iwf.induct)
+  apply (case_tac x)
+  apply (auto elim!: it_paths_ConsE)
+  apply force
+  done
+
+inductive_set hyps_along for t "is" where
+ "prefixeq (is'@[i]) is \<Longrightarrow>
+  hyps (iNodeOf (tree_at t is')) h = Some i \<Longrightarrow>
+  subst (iSubst  (tree_at t is')) (freshen (iAnnot (tree_at t is')) (labelsOut (iNodeOf (tree_at t is')) h)) \<in> hyps_along t is"
+
+lemma hyps_along_Nil[simp]: "hyps_along t [] = {}"
+  by (auto simp add: hyps_along.simps)
+
+lemma prefixeq_app_Cons_elim:
+  assumes "prefixeq (xs@[y]) (z#zs)"
+  obtains "xs = []" and "y = z"
+   | xs' where "xs = z#xs'" and "prefixeq (xs'@[y]) zs"
+using assms by (cases xs) auto
+
+lemma prefixeq_app_Cons_simp:
+  "prefixeq (xs@[y]) (z#zs) \<longleftrightarrow> (xs = [] \<and> y = z \<or> xs = z#tl xs \<and> prefixeq (tl xs@[y]) zs)"
+ by (cases xs) auto
+
+lemma hyps_along_Cons:
+  assumes "i#is \<in> it_paths t"
+  shows "hyps_along t (i#is) =
+    (\<lambda>h. subst (iSubst t) (freshen (iAnnot t) (labelsOut (iNodeOf t) h))) ` fset (hyps_for (iNodeOf t) i)
+    \<union> hyps_along (the (iAnts t i)) is" (is "?S1 = ?S2 \<union> ?S3")
+proof-
+  from assms
+  obtain t' where "i |\<in>| inPorts (iNodeOf t)" and [simp]: "iAnts t i = Some t'" and "is \<in> it_paths t'"
+    by (auto elim: it_paths_ConsE)
+
+  show ?thesis
+  proof (rule; rule)
+    fix x
+    assume "x \<in> hyps_along t (i # is)"
+    then obtain is' i' h where
+      "prefixeq (is'@[i']) (i#is)"
+      and "hyps (iNodeOf (tree_at t is')) h = Some i'"
+      and [simp]: "x = subst (iSubst  (tree_at t is')) (freshen (iAnnot (tree_at t is')) (labelsOut (iNodeOf (tree_at t is')) h))"
+    by (auto elim: hyps_along.cases)
+    from this(1)
+    show "x \<in> ?S2 \<union> ?S3"
+    proof(cases rule: prefixeq_app_Cons_elim)
+      assume "is' = []" and "i' = i"
+      with `hyps (iNodeOf (tree_at t is')) h = Some i'`
+      have "x \<in> ?S2" by auto
+      thus ?thesis..
+    next
+      fix is''
+      assume [simp]: "is' = i # is''" and "prefixeq (is'' @ [i']) is"
+
+      from `hyps (iNodeOf (tree_at t is')) h = Some i'`
+      have "hyps (iNodeOf (tree_at t' is'')) h = Some i'" by simp
+
+      from hyps_along.intros[OF `prefixeq (is'' @ [i']) is` this]
+      have "subst (iSubst (tree_at t' is'')) (freshen (iAnnot (tree_at t' is'')) (labelsOut (iNodeOf (tree_at t' is'')) h))  \<in> hyps_along t' is".
+      hence "x \<in> ?S3" by simp
+      thus ?thesis..
+    qed
+  next
+    fix x
+    assume "x \<in> ?S2 \<union> ?S3"
+    thus "x \<in> ?S1"
+    proof
+      have "prefixeq ([]@[i]) (i#is)" by simp
+      
+      assume "x \<in> ?S2"
+      then obtain h where "h |\<in>| hyps_for (iNodeOf t) i"
+        and [simp]: "x = subst (iSubst t) (freshen (iAnnot t) (labelsOut (iNodeOf t) h))" by auto
+      from this(1)
+      have "hyps (iNodeOf (tree_at t [])) h = Some i" by simp
+      
+      from hyps_along.intros[OF `prefixeq ([]@[i]) (i#is)` this]
+      show "x \<in> hyps_along t (i # is)" by simp
+    next
+      assume "x \<in> ?S3"
+      thus "x \<in> ?S1"
+        apply (auto simp add: hyps_along.simps)
+        apply (rule_tac x = "i#is'" in exI)
+        apply auto
+        done
+    qed
+  qed
+qed
+
+lemma iwf_hyps_exist:
+  assumes "iwf lc it (fst (root ts))"
+  assumes "is \<in> it_paths it"
+  assumes "tree_at it is = (HNode i s)"
+  assumes "fst (fst (root ts)) |\<subseteq>| ass_forms"
+  shows "subst s (freshen i anyP) \<in> hyps_along it is"
+proof-
+  from assms(1,2,3)
+  have "subst s (freshen i anyP) \<in> hyps_along it is 
+     \<or> subst s (freshen i anyP) |\<in>| fst (fst (root ts))
+       \<and> subst s (freshen i anyP) |\<notin>| ass_forms"
+  proof(induction arbitrary: "is" rule: iwf.induct)
+    case (iwf n p ants s' i' \<Gamma> c "is")
+   
+    show ?case
+    proof(cases "is")
+      case Nil
+      with `tree_at (INode n p i' s' ants) is = HNode i s`
+      show ?thesis by auto
+    next
+      case (Cons ip "is'")
+      with `is \<in> it_paths (INode n p i' s' ants)`
+      obtain it where "ip |\<in>| inPorts n" and [simp]: "ants ip = Some it" and "is' \<in> it_paths it"
+        by (auto elim: it_paths_ConsE)
+
+      let ?\<Gamma>' = "(\<lambda>h. subst s' (freshen i' (labelsOut n h))) |`| hyps_for n ip"
+      
+      from `tree_at (INode n p i' s' ants) is = HNode i s`
+      have "tree_at it is' = HNode i s" using Cons `ants ip = Some it` by simp
+
+      from  iwf.IH[OF `ip |\<in>| _`] `ants ip = Some it` `is' \<in> it_paths it` this
+      have  "subst s (freshen i anyP) \<in> hyps_along it is'
+        \<or> subst s (freshen i anyP) |\<in>| ?\<Gamma>' |\<union>| \<Gamma> \<and> subst s (freshen i anyP) |\<notin>| ass_forms"
+        by auto
+      moreover
+      from  `is \<in> it_paths (INode n p i' s' ants)`
+      have "hyps_along (INode n p i' s' ants) is = fset ?\<Gamma>' \<union> hyps_along it is'"
+        using `is = _` by (simp add: hyps_along_Cons)
+      ultimately
+      show ?thesis by auto
+    qed
+  next
+    case (iwfH c  \<Gamma> s' i' "is")
+    hence [simp]: "is = []" "i' = i" "s' = s" by simp_all
+    from `c = subst s' (freshen i' anyP)` `c |\<in>| \<Gamma>` `c |\<notin>| ass_forms`
+    show ?case by simp
+  qed
+  with assms(4)
+  show ?thesis by blast
+qed
+
+fun fv_entailment :: "'form entailment \<Rightarrow> 'var annotated set" where
+  "fv_entailment (\<Gamma> \<turnstile> c) = Union (fv ` fset \<Gamma>) \<union> fv c"
+
+definition hyp_port_for' where
+  "hyp_port_for' t is f = (SOME x.
+   (case x of (is', i, h) \<Rightarrow> 
+      prefixeq (is' @ [i]) is \<and>
+      hyps (iNodeOf (tree_at t is')) h = Some i \<and>
+      f = subst (iSubst  (tree_at t is')) (freshen (iAnnot (tree_at t is')) (labelsOut (iNodeOf (tree_at t is')) h))
+   ))"
+
+lemma hyp_port_for_spec':
+  assumes "f \<in> hyps_along t is"
+  shows "(case hyp_port_for' t is f of (is', i, h) \<Rightarrow> 
+      prefixeq (is' @ [i]) is \<and>
+      hyps (iNodeOf (tree_at t is')) h = Some i \<and>
+      f = subst (iSubst  (tree_at t is')) (freshen (iAnnot (tree_at t is')) (labelsOut (iNodeOf (tree_at t is')) h)))"
+using assms unfolding hyps_along.simps hyp_port_for'_def by -(rule someI_ex, blast)
+
+definition hyp_port_path_for where "hyp_port_path_for t is f = fst (hyp_port_for' t is f)"
+definition hyp_port_i_for where "hyp_port_i_for t is f = fst (snd (hyp_port_for' t is f))"
+definition hyp_port_h_for where "hyp_port_h_for t is f = snd (snd (hyp_port_for' t is f))"
+
+lemma hyp_port_prefixeq:
+  assumes "f \<in> hyps_along t is"
+  shows "prefixeq (hyp_port_path_for t is f@[hyp_port_i_for t is f]) is"
+using hyp_port_for_spec'[OF assms] unfolding hyp_port_path_for_def hyp_port_i_for_def by auto
+
+lemma hyp_port_prefix:
+  assumes "f \<in> hyps_along t is"
+  shows "prefix (hyp_port_path_for t is f) is"
+using hyp_port_prefixeq[OF assms] by (simp add: prefixI' prefix_order.dual_order.strict_trans1)
+
+lemma hyp_port_hyps:
+  assumes "f \<in> hyps_along t is"
+  shows "hyps (iNodeOf (tree_at t (hyp_port_path_for t is f))) (hyp_port_h_for t is f) = Some (hyp_port_i_for t is f)"
+using hyp_port_for_spec'[OF assms] unfolding hyp_port_path_for_def hyp_port_i_for_def hyp_port_h_for_def by auto
+
+lemma hyp_port_outPort:
+  assumes "f \<in> hyps_along t is"
+  shows "(hyp_port_h_for t is f) |\<in>| outPorts (iNodeOf (tree_at t (hyp_port_path_for t is f)))"
+using hyps_correct[OF hyp_port_hyps[OF assms]]..
+
+lemma hyp_port_eq:
+  assumes "f \<in> hyps_along t is"
+  shows "f = subst (iSubst (tree_at t (hyp_port_path_for t is f))) (freshen (iAnnot (tree_at t (hyp_port_path_for t is f))) (labelsOut (iNodeOf (tree_at t (hyp_port_path_for t is f))) (hyp_port_h_for t is f)))"
+using hyp_port_for_spec'[OF assms] unfolding hyp_port_path_for_def hyp_port_i_for_def hyp_port_h_for_def by auto
+
+
+lemma iwf_outPort: 
+  assumes "iwf fc t ent"
+  assumes "x \<in> it_paths t"
+  shows "Reg (iOutPort (tree_at t x)) |\<in>| outPorts (iNodeOf (tree_at t x))"
+using assms
+  apply (induction arbitrary: x rule: iwf.induct)
+  apply (case_tac x)
+  apply (auto elim!: it_paths_ConsE)
+  apply force
+  done
+
+fun inits where
+  "inits [] = [[]]"
+| "inits (i#is) = [] # map (op # i) (inits is)"
+
+lemma inits_Snoc[simp]:
+  "inits (is@[i]) = inits is @ [is@[i]]"
+by (induction "is") auto
+
+lemma inits_eq_Snoc:
+  "inits is = xs @ [x] \<longleftrightarrow> (is = [] \<and> xs = [] \<or> (\<exists> i is'. is = is'@[i] \<and> xs = inits is')) \<and> x = is"
+by (cases "is" rule: rev_cases) auto
+
+lemma in_set_inits[simp]: "is' \<in> set (inits is) \<longleftrightarrow> prefixeq is' is"
+  by (induction "is'" arbitrary: "is"; case_tac "is"; auto)
+
+
+
+
+  text {*
+  Like local_iwf, but every name occuring in a substitution has
+  is either in the conclusion of the rule, or created by this rule.
+  *}
+
+  inductive global_fresh_check :: "('preform, 'rule, 'subst, 'form) fresh_check" where
+    "ran_fv s \<subseteq> fv_entailment (\<Gamma> \<turnstile> c) \<union> range (freshenV i) \<Longrightarrow> global_fresh_check n i s (\<Gamma> \<turnstile> c)"
+
+  abbreviation "global_iwf \<equiv> iwf global_fresh_check"
+
+  definition globalize :: "('preform,'rule,'subst,'var) itree \<Rightarrow> ('preform,'rule,'subst,'var) itree" where
+    "globalize = undefined"
+
+
+  lemma globalized:
+    assumes "tfinite t" and "wf t"
+    assumes "local_iwf it' (fst (root t))"
+    shows "global_iwf (globalize it') (fst (root t))"
+    sorry
+
+  lemma it_paths_globalize:
+    "it_paths (globalize it) = it_paths it"
+    sorry
+
+end   
+
+end
